Projects/Util/Data/LeafTrie/Raw0.lean
@@ -4,15 +4,17 @@ section Logic
 
 variable {α β γ : Type*}
 
-theorem dite_true_eq! : @dite α True = λ _ f _ => f trivial := by
-  funext; simp
-
-theorem dite_false_eq! : @dite α False = λ _ _ g => g not_false := by
-  funext; simp
-
 -- #check 0 #exit
 
 end Logic
+
+section Order
+
+variable {α β γ : Type*}
+
+-- #check 0 #exit
+
+end Order
 
 namespace Nat
 
@@ -32,20 +34,6 @@ namespace List
 
 variable {α β γ : Type*}
 variable {xs ys zs : List α}
-
-theorem flatMap_eq_flatten_map {f : α → List β} : xs.flatMap f = (xs.map f).flatten := by
-  exact flatMap_def
-
-theorem foldr_fn_append_eq_flatMap {f : α → List β} {zs} :
-xs.foldr (λ x acc => f x ++ acc) zs = xs.flatMap f ++ zs := by
-  cases xs <;> simp; rfl
-
-theorem map_eq_map_attach {f : α → β} : xs.map f = xs.attach.map (λ x => f x.1) := by
-  simp
-
-@[simp]
-theorem getElem?_singleton_eq_some_iff {x y : α} {i} : [x][i]? = some y ↔ i = 0 ∧ x = y := by
-  grind
 
 -- #check 0 #exit
 
@@ -67,147 +55,6 @@ variable {α : Type*} {β : α → Type*} {γ : Type*}
 variable [hh₁ : DecidableEq α] [hh₂ : Hashable α]
 variable {mp : Raw α β} {wf : mp.WF}
   {f : γ → (i : α) → (x : β i) → mp.get? i = some x → γ} {z : γ}
-
-omit hh₁ hh₂ in @[simp]
-theorem assocList_foldr_nil {f : (x : α) → β x → γ → γ} {z} :
-Internal.AssocList.nil.foldr f z = z := rfl
-
-omit hh₁ hh₂ in @[simp]
-theorem assocList_foldr_cons {f : (x : α) → β x → γ → γ} {k x z} {bs} :
-(Internal.AssocList.cons k x bs).foldr f z =
-f k x (bs.foldr f z) := rfl
-
-omit hh₁ hh₂ in @[simp]
-theorem assocList_foldr_eq_foldr_toList
-{bs : Internal.AssocList α β} {f : (x : α) → β x → γ → γ} {z} :
-bs.foldr f z = bs.toList.foldr (λ x => f x.1 x.2) z := by
-  induction bs generalizing z <;> simp
-  nm k x bs ih; grind
-
-omit hh₁ hh₂ in
-theorem foldr_foldr_eq_foldr_flatMap_buckets_list {bs : List (Internal.AssocList α β)} :
-bs.foldr (λ x y => DHashMap.Internal.AssocList.foldr
-(λ a b d => Sigma.mk a b :: d) y x) [] = bs.flatMap (·.toList) := by
-  simp; rfl
-
-omit hh₁ hh₂ in
-theorem foldr_foldr_eq_foldr_flatMap_buckets_array {bs : Array (Internal.AssocList α β)} :
-bs.foldr (λ x y => DHashMap.Internal.AssocList.foldr
-(λ a b d => Sigma.mk a b :: d) y x) [] = bs.toList.flatMap (·.toList) := by
-  rcases bs with ⟨bs⟩
-  simp only [assocList_foldr_eq_foldr_toList, Sigma.eta, List.foldr_cons_eq_append',
-    List.size_toArray, List.foldr_toArray', List.foldr_append_eq_append, List.append_nil,
-    List.flatMap_eq_flatten_map]
-
-omit hh₁ hh₂ in @[simp]
-theorem assocList_foldrM_Id_eq_foldr_toList
-{bs : Internal.AssocList α β} {f : (x : α) → β x → γ → γ} {z} :
-bs.foldrM (m := Id) f z = bs.toList.foldr (λ x => f x.1 x.2) z :=
-  assocList_foldr_eq_foldr_toList
-
-omit hh₁ hh₂ in open Classical in
-theorem assocList_foldrM_eq!.{u, v, w} : @Internal.AssocList.foldrM.{w, v, u, w} =
-λ (α : Type u) (β : α → Type v) (γ : Type w) (m : Type w → Type w) [H : Monad m]
-(f : (x : α) → β x → γ → m γ) (z : γ) (bs : Internal.AssocList α β) =>
-if h : m = Id ∧ H ≍ Id.instMonad then by
-  rcases h with ⟨rfl, h⟩
-  exact bs.toList.foldr (λ x => f x.1 x.2) z
-else bs.foldrM f z := by
-  funext α β γ m H f z bs
-  simp only [right_eq_dite_iff, forall_and_index]
-  rintro rfl
-  revert f
-  simp only [Id]
-  rintro f rfl
-  simp [-Id.instMonad]
-  generalize_proofs H
-  cases H
-  rfl
-
-omit hh₁ hh₂ in
-theorem toList_eq_flatMap_buckets : mp.toList = mp.buckets.toList.flatMap (·.toList) := by
-  rw [toList, Internal.foldRev, Internal.foldRevM, ←Array.foldrM_toList]
-  generalize mp.buckets.toList = xs; clear! mp
-  simp only [Id.run, pure, assocList_foldrM_Id_eq_foldr_toList, Sigma.eta,
-    List.foldr_cons_eq_append']
-  rw [List.foldrM_eq_foldr]; unfold Id Id.instMonad
-  simp only [pure, bind, List.foldr_append_eq_append, List.append_nil]; rfl
-
-omit hh₂ in
-theorem of_getCast?_eq_some {xs : Internal.AssocList α β} {k x}
-(h : xs.getCast? k = some x) : ⟨k, x⟩ ∈ xs.toList := by
-  induction xs generalizing k x <;> simp at h ⊢
-  nm r y xs ih
-  rw [Internal.List.getValueCast?_cons] at h
-  simp at h
-  split_ifs at h with h₁
-  · subst h₁
-    simp at h
-    subst h
-    simp
-  right
-  simp_rw [Internal.AssocList.getCast?_eq] at ih
-  tauto
-
-theorem distinct_keys_of_mem_buckets {xs} (wf : mp.WF) (h : xs ∈ mp.buckets) :
-∀ k x y, ⟨k, x⟩ ∈ xs.toList → ⟨k, y⟩ ∈ xs.toList → x = y := by
-  intro k x y h₁ h₂
-  generalize h₃ : DHashMap.mk mp wf = mp₁
-  have h₄ : ∀ ⦃z⦄, z ∈ xs.toList → z ∈ mp₁.toList
-  · intro z hz
-    rw [DHashMap.toList, toList_eq_flatMap_buckets]
-    simp
-    grind
-  replace h₁ := h₄ h₁
-  replace h₂ := h₄ h₂
-  rw [DHashMap.mem_toList_iff_get?_eq_some] at h₁ h₂
-  grind
-
-theorem distinct_keys_of_mem_toList_buckets {xs} (wf : mp.WF) (h : xs ∈ mp.buckets.toList) :
-∀ k x y, ⟨k, x⟩ ∈ xs.toList → ⟨k, y⟩ ∈ xs.toList → x = y := by
-  simp at h; exact distinct_keys_of_mem_buckets wf h
-
-omit hh₂ in
-theorem getCast?_eq_some_iff {xs : Internal.AssocList α β} {k x}
-(h : ∀ k x y, ⟨k, x⟩ ∈ xs.toList → ⟨k, y⟩ ∈ xs.toList → x = y) :
-xs.getCast? k = some x ↔ ⟨k, x⟩ ∈ xs.toList := by
-  constructor; use of_getCast?_eq_some
-  rw [Internal.AssocList.getCast?_eq]
-  intro h₁
-  induction xs generalizing k x <;> simp at h₁
-  nm r y xs ih
-  rcases h₁ with ⟨rfl, h₁⟩ | h₁
-  · simp at h₁
-    simp [h₁]
-  simp
-  rw [Internal.List.getValueCast?_cons]
-  simp
-  split_ifs with h₂
-  · subst h₂
-    simp
-    tauto
-  apply ih _ h₁
-  tauto
-
-theorem getCast?_eq_some_iff_of_mem_buckets {xs k x} (wf : mp.WF)
-(h : xs ∈ mp.buckets) : xs.getCast? k = some x ↔ ⟨k, x⟩ ∈ xs.toList :=
-  getCast?_eq_some_iff # distinct_keys_of_mem_buckets wf h
-
-theorem get?_eq_some_iff_mem_toList {k x} (wf : mp.WF) :
-mp.get? k = some x ↔ ⟨k, x⟩ ∈ mp.toList := by
-  generalize h₁ : DHashMap.mk mp wf = mp₁
-  convert_to mp₁.get? k = some x ↔ ⟨k, x⟩ ∈ mp₁.toList
-  · subst h₁
-    rw [get?, DHashMap.get?]
-    grind
-  · subst h₁
-    rfl
-  simp
-
-omit hh₁ hh₂ in @[simp]
-theorem assocList_toList_eq_nil_iff {xs : Internal.AssocList α β} :
-xs.toList = [] ↔ xs = .nil := by
-  unfold Internal.AssocList.toList; split <;> simp
 
 -- #check 0 #exit
 
@@ -284,7 +131,7 @@ t.depthAux < (node mp : Raw₀ α β).depthAux := by
   simp only [List.rec_eq_foldr, List.foldr_max_eq_max?_map]
   generalize hf : (λ (x : DHashMap.Internal.AssocList α # λ _ => Raw₀ α β) => _) = f
   change (λ x => (x.toList.map (λ x => x.snd.depthAux)).max?.elim 0 (max 0)) = f at hf
-  simp at hf ⊢
+  simp [-List.elim_max?_id_eq_max!] at hf ⊢
   rw [List.max?_eq_some_max]
   rotate_left
   · simp
@@ -296,7 +143,7 @@ t.depthAux < (node mp : Raw₀ α β).depthAux := by
   simp
   apply List.le_max_of_le_mem
   subst hf hb
-  simp
+  simp [-List.elim_max?_id_eq_max!]
   simp [DHashMap.Raw.get?] at h
   choose h₁ h₂ using h
   simp [DHashMap.Internal.Raw₀.get?] at h₂
@@ -309,7 +156,7 @@ t.depthAux < (node mp : Raw₀ α β).depthAux := by
   have h₄ := Internal.List.getValueCast_mem h₂
   rw [h₃] at h₄
   use b
-  simp [←hb]
+  simp [-List.elim_max?_id_eq_max!, ←hb]
   rw [List.max?_eq_some_max]
   rotate_left
   · simp only [ne_eq, List.map_eq_nil_iff]; grind
@@ -420,119 +267,56 @@ theorem wf_node_iff {mp} : (node mp : Raw₀ α β).WF ↔
 mp.WF ∧ ∀ k t₁, mp.get? k = some t₁ → t₁.WF := by
   rw [wf_iff]; simp
 
--- theorem depthAux_eq_depth [wf : t.WF] : t.depthAux = t.depth := by
---   classical
---   suffices h : ∀ (wf : t.WF), t.depthAux = t.depth; tauto
---   apply @t.rec' (wf := wf) (γ := λ t => ∀ (wf : t.WF), t.depthAux = t.depth) <;> clear! t
---   ·
---     intro x wf
---     simp
---   intro mp wf₁ ih wf₂
---   unfold depthAux
---   simp [rec_3_eq, rec_4_eq]
---   generalize hb : mp.2.toList = bs
---   simp only [List.rec_eq_foldr, List.foldr_max_eq_max?_map]
---   generalize hf : (λ (x : DHashMap.Internal.AssocList α # λ _ => Raw₀ α β) => _) = f
---   change (λ x => (x.toList.map (λ x => x.snd.depthAux)).max?.elim 0 (max 0)) = f at hf
---   simp at hf ⊢
---   
---   rw [wf_node_iff] at wf₂
---   obtain ⟨wf₂, wf₃⟩ := wf₂
---   
---   -- by_cases h₁ : mp.isEmpty
---   -- ·
---   --   rw [←DHashMap.Raw.toList_eq_nil_iff_isEmpty wf₂] at h₁
---   -- 
---   -- rw [List.max?_eq_some_max]
---   -- rotate_left
---   -- · simp
---   --   rintro rfl
---   --   simp at hb
---   --   simp [DHashMap.Raw.get?] at h
---   --   obtain ⟨h₁, h₂⟩ := h
---   --   simp [hb] at h₁
---   -- simp
---   -- apply List.le_max_of_le_mem
---   -- subst hf hb
---   
---   rw [depth_node, Nat.add_comm 1]
---   simp
---   
---   rw [DHashMap.Raw.foldWith_eq_foldlWith_toList, List.foldlWith_max_eq_max?_mapWith]
---   simp
---   
---   rw! [DHashMap.Raw.toList, DHashMap.Raw.Internal.foldRev,
---     DHashMap.Raw.Internal.foldRevM]
---   simp [pure, Id.run]
---   
---   trans
---     ((mp.buckets.foldr (λ x1 x2 => DHashMap.Internal.AssocList.foldrM (m := Id)
---     (λ a b d => ⟨a, b⟩ :: (d : List ((_ : α) × Raw₀ α β))) x2 x1) []).mapWith
---           λ x h =>
---           haveI : x.2.WF := (
---             by
---               simp only [DHashMap.Raw.assocList_foldrM_Id_eq_foldr_toList, Sigma.eta,
---                 List.foldr_cons_eq_append'] at h
---               rw [←Array.foldr_toList, hb] at h
---               dsimp [Id] at h
---               rw [List.foldr_fn_append_eq_flatMap] at h
---               simp at h
---               obtain ⟨xs, h₁, h₂⟩ := h
---               rcases x with ⟨x, t₁⟩
---               dsimp
---               apply wf₃ x t₁
---               rw [DHashMap.Raw.get?_eq_some_iff_mem_toList wf₂]
---               rw [DHashMap.Raw.toList_eq_flatMap_buckets]
---               simp; grind
---           ); x.2.depth).max?.elim
---     0 id
--- 
--- -- #check 0 #exit
---   
---   on_goal 2 => congr
---   rw [List.mapWith_eq_map]
---   simp
---   split_ifs with h₁
---   ·
---     simp at h₁ ⊢
---     unfold Id at h₁
---     rw [←Array.foldr_toList] at h₁
---     rw [List.foldr_fn_append_eq_flatMap] at h₁
---     simp at h₁
---     clear ih; nm x; clear x
---     clear wf₂
---     have h₂ : bs.map f = bs.map (λ _ => 0)
---     ·
---       rw [List.map_eq_map_iff]
---       subst hf
---       simp
---       intro b₁ hb₁
---       specialize h₁ b₁ (by grind)
---       simp [h₁]
---     rw [h₂]
---     clear! f
---     simp
---     rw [List.max?_replicate]
---     grind
---   
---   unfold Id Id.instMonad
---   iterate 2 rw! [←Array.foldr_toList]
---   iterate 2 rw! [List.foldr_fn_append_eq_flatMap]
---   simp
---   rw! [←DHashMap.Raw.toList_eq_flatMap_buckets]
---   generalize hb₁ : Array.mk bs = bs₁
---   subst hb
---   rename' bs₁ => bs
---   simp at hb₁
---   simp [hb₁]
---   clear h₁
---   nm x; clear x
---   
---   rw! [DHashMap.Raw.toList_eq_flatMap_buckets, hb₁]
---   rw! [List.map_flatMap, List.map_eq_flatMap, List.flatMap, List.flatMap]
---   nth_rw 1 [List.map_eq_map_attach]
---   nth_rw 2 [List.map_eq_map_attach]
---   
---   congr 1
---   
---   sorry
+theorem depthAux_node {mp} : (node mp : Raw₀ α β).depthAux =
+1 + mp.toList.foldl (init := 0) λ acc x => max acc # x.2.depthAux := by
+  rw [depthAux]
+  simp [rec_3_eq, rec_4_eq]
+  rw [List.rec_eq_foldr]
+  change mp.2.toList.foldr (λ x =>
+    max (x.toList.rec 0 (λ x xs acc => max x.snd.depthAux acc))) 0 + 1 = _
+  simp_rw [List.rec_eq_foldr]
+  rw [List.foldl_eq_foldl_map (·.snd.depthAux) max (by grind)]
+  rw [add_comm 1]; congr 1
+  rw [←List.foldr_eq_foldl']
+  rw [DHashMap.Raw.toList_eq_flatMap_buckets]
+  generalize mp.buckets.toList = bs
+  clear! mp
+  rw [List.foldr_eq_foldr_map (·.toList.foldr (λ x => max x.2.depthAux) 0) max (by grind)]
+  rw [List.map_flatMap]
+  simp [List.foldr_max_eq_max?_map]
+  generalize hf : (λ (xs : DHashMap.Internal.AssocList α (λ _ => Raw₀ α β)) =>
+    xs.toList.map (λ x => x.2.depthAux)) = f
+  trans bs.map (λ x => f x |>.max!) |>.max!
+  · subst hf; rfl
+  clear hf
+  rw [List.flatMap_eq_flatten_map]
+  rw [List.max!_flatten]
+  simp
+
+theorem depthAux_node' {mp} (wf : (node mp : Raw₀ α β).WF) :
+(node mp).depthAux = 1 + mp.foldWith wf.mp (z := 0)
+λ acc _ t _ => max acc # t.depthAux := by
+  classical
+  rw [depthAux_node]
+  simp
+  rw [DHashMap.Raw.foldWith_eq_foldl_toList]
+  rw [←List.foldl_attach]
+  nth_rw 2 [←List.foldl_attach]
+  congr
+  funext i x
+  rcases x with ⟨⟨k, t₁⟩, h⟩
+  simp [h]
+
+theorem depthAux_eq_depth [wf : t.WF] : t.depthAux = t.depth := by
+  classical
+  suffices h : ∀ (wf : t.WF), t.depthAux = t.depth; tauto
+  apply @t.rec' (wf := wf) (γ := λ t => ∀ (wf : t.WF), t.depthAux = t.depth) <;> clear! t
+  · intro x wf
+    simp
+  intro mp wf₁ ih wf₂
+  rw [depthAux_node' wf₂, depth_node]
+  simp
+  congr
+  funext i x t₁ h
+  specialize ih x t₁ h (wf₂.get? h)
+  rw [ih]
